src/lib/utils/DY.Lib.SplitFunction.fst
@@ -70,10 +70,7 @@ open Comparse //for_allP, for_allP_eq
 
 /// The parameters of the split function methodology.
 
-noeq type split_function_input_values = {
-  // Input type for the global function
-  tagged_data_t: Type;
-
+noeq type split_function_parameters = {
   // Functions to model set of tags
   tag_set_t: Type;
   tag_t: Type;
@@ -83,6 +80,8 @@ noeq type split_function_input_values = {
     tag:tag_t -> tag_set_1:tag_set_t -> tag_set_2:tag_set_t -> Lemma
     (~(tag_set_1 `is_disjoint` tag_set_2 /\ tag `tag_belong_to` tag_set_1 /\ tag `tag_belong_to` tag_set_2));
 
+  // Input type for the global function
+  tagged_data_t: Type;
 
   // Input type for the local functions
   raw_data_t: Type;
@@ -92,7 +91,7 @@ noeq type split_function_input_values = {
 
   // We can decode the global function input
   // into a tag and a local function input
-  decode_tagged_data: tagged_data_t -> Tot (option (tag_t & raw_data_t));
+  decode_tagged_data: tagged_data_t -> option (tag_t & raw_data_t);
 
   // Types for the local functions and the global function
   local_fun_t: Type;
@@ -114,45 +113,45 @@ noeq type split_function_input_values = {
 /// Do a global function contain some given local function with some set of tags?
 /// This will be a crucial precondition for the correctness theorem `local_eq_global_lemma`.
 
-val has_local_fun: func:split_function_input_values -> func.global_fun_t -> (func.tag_set_t & func.local_fun_t) -> prop
-let has_local_fun func global_fun (tag_set, tagged_local_fun) =
+val has_local_fun: params:split_function_parameters -> params.global_fun_t -> (params.tag_set_t & params.local_fun_t) -> prop
+let has_local_fun params global_fun (tag_set, tagged_local_fun) =
   forall tagged_data.
-    match func.decode_tagged_data tagged_data with
+    match params.decode_tagged_data tagged_data with
     | Some (tag, raw_data) ->
-      tag `func.tag_belong_to` tag_set ==> (func.apply_global_fun global_fun tagged_data == func.apply_local_fun tagged_local_fun raw_data)
+      tag `params.tag_belong_to` tag_set ==> (params.apply_global_fun global_fun tagged_data == params.apply_local_fun tagged_local_fun raw_data)
     | None -> True
 
 /// Returns the first local function associated with a tag set containing `tag`, if it exists.
 /// In practice, only one tag set may contain `tag` because tag sets are mutually disjoint
 /// (c.f. precondition of `mk_global_fun_correct`).
 /// In that case, this function returns the *unique* local function associated with a tag set containing `tag`.
-val find_local_fun: func:split_function_input_values -> list (func.tag_set_t & func.local_fun_t) -> func.tag_t -> option func.local_fun_t
-let rec find_local_fun func tagged_local_funs tag =
+val find_local_fun: params:split_function_parameters -> list (params.tag_set_t & params.local_fun_t) -> params.tag_t -> option params.local_fun_t
+let rec find_local_fun params tagged_local_funs tag =
   match tagged_local_funs with
   | [] -> None
   | (h_tag_set, h_local_fun)::t_tagged_local_funs -> (
-    if tag `func.tag_belong_to` h_tag_set then
+    if tag `params.tag_belong_to` h_tag_set then
       Some h_local_fun
     else
-      find_local_fun func t_tagged_local_funs tag
+      find_local_fun params t_tagged_local_funs tag
   )
 
-val mk_global_fun_aux: func:split_function_input_values -> list (func.tag_set_t & func.local_fun_t) -> func.tagged_data_t -> func.output_t
-let mk_global_fun_aux func tagged_local_funs tagged_data =
-  match func.decode_tagged_data tagged_data with
+val mk_global_fun_aux: params:split_function_parameters -> list (params.tag_set_t & params.local_fun_t) -> params.tagged_data_t -> params.output_t
+let mk_global_fun_aux params tagged_local_funs tagged_data =
+  match params.decode_tagged_data tagged_data with
   | Some (tag_set, raw_data) -> (
-    match find_local_fun func tagged_local_funs tag_set with
-    | Some tagged_local_fun -> func.apply_local_fun tagged_local_fun raw_data
-    | None -> func.apply_global_fun func.default_global_fun tagged_data
+    match find_local_fun params tagged_local_funs tag_set with
+    | Some tagged_local_fun -> params.apply_local_fun tagged_local_fun raw_data
+    | None -> params.apply_global_fun params.default_global_fun tagged_data
   )
-  | None -> func.apply_global_fun func.default_global_fun tagged_data
+  | None -> params.apply_global_fun params.default_global_fun tagged_data
 
 /// Given a list of tags and local functions, create the global function.
 
 [@@"opaque_to_smt"]
-val mk_global_fun: func:split_function_input_values -> list (func.tag_set_t & func.local_fun_t) -> func.global_fun_t
-let mk_global_fun func tagged_local_funs =
-  func.mk_global_fun (mk_global_fun_aux func tagged_local_funs)
+val mk_global_fun: params:split_function_parameters -> list (params.tag_set_t & params.local_fun_t) -> params.global_fun_t
+let mk_global_fun params tagged_local_funs =
+  params.mk_global_fun (mk_global_fun_aux params tagged_local_funs)
 
 val memP_map:
   #a:Type -> #b:Type ->
@@ -167,58 +166,58 @@ let rec memP_map #a #b f l x =
     introduce x =!= h ==> List.Tot.memP (f x) (List.Tot.map f t)
     with _. memP_map f t x
 
-val all_disjoint : #a:Type -> (a -> a -> prop) -> list a -> prop
-let rec all_disjoint #a disj l =
+val for_all_pairsP : #a:Type -> (a -> a -> prop) -> list a -> prop
+let rec for_all_pairsP #a disj l =
   match l with
   | [] -> True
-  | h::t -> (for_allP (disj h) t) /\ all_disjoint disj t
+  | h::t -> (for_allP (disj h) t) /\ for_all_pairsP disj t
 
 val mk_global_fun_correct_aux:
-  func:split_function_input_values -> tagged_local_funs:list (func.tag_set_t & func.local_fun_t) -> tag_set:func.tag_set_t -> local_fun:func.local_fun_t -> tag:func.tag_t ->
+  params:split_function_parameters -> tagged_local_funs:list (params.tag_set_t & params.local_fun_t) -> tag_set:params.tag_set_t -> local_fun:params.local_fun_t -> tag:params.tag_t ->
   Lemma
   (requires
-    all_disjoint (func.is_disjoint) (List.Tot.map fst tagged_local_funs) /\
-    tag `func.tag_belong_to` tag_set /\
+    for_all_pairsP (params.is_disjoint) (List.Tot.map fst tagged_local_funs) /\
+    tag `params.tag_belong_to` tag_set /\
     List.Tot.memP (tag_set, local_fun) tagged_local_funs
   )
-  (ensures find_local_fun func tagged_local_funs tag == Some local_fun)
-let rec mk_global_fun_correct_aux func tagged_local_funs tag_set tagged_local_fun tag =
+  (ensures find_local_fun params tagged_local_funs tag == Some local_fun)
+let rec mk_global_fun_correct_aux params tagged_local_funs tag_set tagged_local_fun tag =
   match tagged_local_funs with
   | [] -> ()
   | (h_tag_set, h_tagged_local_fun)::t_tagged_local_funs -> (
-    if tag `func.tag_belong_to` h_tag_set then (
+    if tag `params.tag_belong_to` h_tag_set then (
       introduce (List.Tot.memP (tag_set, tagged_local_fun) t_tagged_local_funs) ==> False with _. (
-        for_allP_eq (func.is_disjoint h_tag_set) (List.Tot.map fst t_tagged_local_funs);
+        for_allP_eq (params.is_disjoint h_tag_set) (List.Tot.map fst t_tagged_local_funs);
         memP_map fst t_tagged_local_funs (tag_set, tagged_local_fun);
-        func.cant_belong_to_disjoint_sets tag h_tag_set tag_set
+        params.cant_belong_to_disjoint_sets tag h_tag_set tag_set
       )
     ) else (
-      mk_global_fun_correct_aux func t_tagged_local_funs tag_set tagged_local_fun tag
+      mk_global_fun_correct_aux params t_tagged_local_funs tag_set tagged_local_fun tag
     )
   )
 
 val mk_global_fun_correct:
-  func:split_function_input_values -> tagged_local_funs:list (func.tag_set_t & func.local_fun_t) -> tag_set:func.tag_set_t -> local_fun:func.local_fun_t ->
+  params:split_function_parameters -> tagged_local_funs:list (params.tag_set_t & params.local_fun_t) -> tag_set:params.tag_set_t -> local_fun:params.local_fun_t ->
   Lemma
   (requires
-    all_disjoint (func.is_disjoint) (List.Tot.map fst tagged_local_funs) /\
+    for_all_pairsP (params.is_disjoint) (List.Tot.map fst tagged_local_funs) /\
     List.Tot.memP (tag_set, local_fun) tagged_local_funs
   )
-  (ensures has_local_fun func (mk_global_fun func tagged_local_funs) (tag_set, local_fun))
-let mk_global_fun_correct func tagged_local_funs tag_set local_fun =
+  (ensures has_local_fun params (mk_global_fun params tagged_local_funs) (tag_set, local_fun))
+let mk_global_fun_correct params tagged_local_funs tag_set local_fun =
   reveal_opaque (`%mk_global_fun) (mk_global_fun);
   introduce
     forall tagged_data.
-      match func.decode_tagged_data tagged_data with
+      match params.decode_tagged_data tagged_data with
       | Some (tag, raw_data) ->
-        tag `func.tag_belong_to` tag_set ==> (func.apply_global_fun (mk_global_fun func tagged_local_funs) tagged_data == func.apply_local_fun local_fun raw_data)
+        tag `params.tag_belong_to` tag_set ==> (params.apply_global_fun (mk_global_fun params tagged_local_funs) tagged_data == params.apply_local_fun local_fun raw_data)
       | None -> True
   with (
-    match func.decode_tagged_data tagged_data with
+    match params.decode_tagged_data tagged_data with
     | Some (tag, raw_data) -> (
-      if tag `func.tag_belong_to` tag_set then (
-        mk_global_fun_correct_aux func tagged_local_funs tag_set local_fun tag;
-        func.apply_mk_global_fun (mk_global_fun_aux func tagged_local_funs) tagged_data
+      if tag `params.tag_belong_to` tag_set then (
+        mk_global_fun_correct_aux params tagged_local_funs tag_set local_fun tag;
+        params.apply_mk_global_fun (mk_global_fun_aux params tagged_local_funs) tagged_data
       ) else ()
     )
     | None -> ()
@@ -230,58 +229,90 @@ let mk_global_fun_correct func tagged_local_funs tag_set local_fun =
 /// (e.g. the function keep the same output when the trace grows.)
 
 val mk_global_fun_eq:
-  func:split_function_input_values -> tagged_local_funs:list (func.tag_set_t & func.local_fun_t) ->
-  tagged_data:func.tagged_data_t ->
+  params:split_function_parameters -> tagged_local_funs:list (params.tag_set_t & params.local_fun_t) ->
+  tagged_data:params.tagged_data_t ->
   Lemma (
-    func.apply_global_fun (mk_global_fun func tagged_local_funs) tagged_data == (
-      match func.decode_tagged_data tagged_data with
+    params.apply_global_fun (mk_global_fun params tagged_local_funs) tagged_data == (
+      match params.decode_tagged_data tagged_data with
       | Some (tag, raw_data) -> (
-        match find_local_fun func tagged_local_funs tag with
-        | Some tagged_local_fun -> func.apply_local_fun tagged_local_fun raw_data
-        | None -> func.apply_global_fun func.default_global_fun tagged_data
+        match find_local_fun params tagged_local_funs tag with
+        | Some tagged_local_fun -> params.apply_local_fun tagged_local_fun raw_data
+        | None -> params.apply_global_fun params.default_global_fun tagged_data
       )
-      | None -> func.apply_global_fun func.default_global_fun tagged_data
+      | None -> params.apply_global_fun params.default_global_fun tagged_data
     )
   )
-let mk_global_fun_eq func tagged_local_funs tagged_data =
+let mk_global_fun_eq params tagged_local_funs tagged_data =
   reveal_opaque (`%mk_global_fun) (mk_global_fun);
-  func.apply_mk_global_fun (mk_global_fun_aux func tagged_local_funs) tagged_data
+  params.apply_mk_global_fun (mk_global_fun_aux params tagged_local_funs) tagged_data
 
 /// If a global function contains some local function,
 /// and the global function input decodes to a tag for this local function,
 /// then the global function is equivalent to the local function on this input.
 
 val local_eq_global_lemma:
-  func:split_function_input_values ->
-  global_fun:func.global_fun_t -> tag_set:func.tag_set_t -> local_fun:func.local_fun_t ->
-  tagged_data:func.tagged_data_t -> tag:func.tag_t -> raw_data:func.raw_data_t ->
+  params:split_function_parameters ->
+  global_fun:params.global_fun_t -> tag_set:params.tag_set_t -> local_fun:params.local_fun_t ->
+  tagged_data:params.tagged_data_t -> tag:params.tag_t -> raw_data:params.raw_data_t ->
   Lemma
   (requires
-    func.decode_tagged_data tagged_data == Some (tag, raw_data) /\
-    tag `func.tag_belong_to` tag_set /\
-    has_local_fun func global_fun (tag_set, local_fun)
+    params.decode_tagged_data tagged_data == Some (tag, raw_data) /\
+    tag `params.tag_belong_to` tag_set /\
+    has_local_fun params global_fun (tag_set, local_fun)
   )
-  (ensures func.apply_global_fun global_fun tagged_data == func.apply_local_fun local_fun raw_data)
-let local_eq_global_lemma func global_fun tag_set tagged_local_fun tagged_data tag raw_data = ()
+  (ensures params.apply_global_fun global_fun tagged_data == params.apply_local_fun local_fun raw_data)
+let local_eq_global_lemma params global_fun tag_set tagged_local_fun tagged_data tag raw_data = ()
 
 /// In the common case where tag disjointness is unequality,
-/// `all_disjoint` is equivalent to the `no_repeats_p` predicate
-/// from F*'s standard library.
+/// the `no_repeats_p` predicate from F*'s standard library
+/// implies `for_all_pairsP unequal`.
+/// It is actually equivalent, but only this implication is useful.
 
 val unequal:
   #a:Type ->
   a -> a -> prop
 let unequal #a x y = x =!= y
 
-val no_repeats_p_implies_all_disjoint:
+val no_repeats_p_implies_for_all_pairsP_unequal:
   #a:Type ->
   l:list a ->
   Lemma
   (requires List.Tot.no_repeats_p l)
-  (ensures all_disjoint unequal l)
-let rec no_repeats_p_implies_all_disjoint #a l =
+  (ensures for_all_pairsP unequal l)
+let rec no_repeats_p_implies_for_all_pairsP_unequal #a l =
   match l with
   | [] -> ()
   | h::t ->
-    no_repeats_p_implies_all_disjoint t;
+    no_repeats_p_implies_for_all_pairsP_unequal t;
     for_allP_eq (unequal h) t
+
+/// In the common case tag sets are simple singletons,
+/// these parameters can be used like this:
+/// {
+///   singleton_split_function_parameters string with
+///   ...
+/// }
+
+let singleton_split_function_parameters (a:eqtype): split_function_parameters = {
+  tag_set_t = a;
+  tag_t = a;
+  is_disjoint = unequal;
+  tag_belong_to = (fun tag tag_set -> tag = tag_set);
+  cant_belong_to_disjoint_sets = (fun tag tag_set1 tag_set2 -> ());
+
+  // everything below should be redefined
+  tagged_data_t = unit;
+  raw_data_t = unit;
+  output_t = unit;
+  decode_tagged_data = (fun x -> None);
+
+  local_fun_t = unit;
+  global_fun_t = unit;
+
+  default_global_fun = ();
+
+  apply_local_fun = (fun lfun x -> ());
+  apply_global_fun = (fun gfun x -> ());
+  mk_global_fun = (fun bare -> ());
+  apply_mk_global_fun = (fun bare x -> ());
+}
